Sorted.v
@@ -3,9 +3,10 @@ Require Export Permutation.
 From sorting Require Export Utils.
 
 Inductive sorted: list nat -> Prop := 
-  | sorted_nil: sorted nil
-  | sorted_1: forall x, sorted (x::nil)
-  | sorted_cons: forall x y l, x <= y -> sorted (y::l) -> sorted (x::y::l).
+  | sorted_nil : sorted nil
+  | sorted_1 : forall (x : nat), sorted (x :: nil)
+  | sorted_cons : forall (x y : nat) (l : list nat),
+      x <= y -> sorted (y :: l) -> sorted (x :: y :: l).
 
 Definition is_a_sorting_algorithm (f: list nat -> list nat) :=
-  forall al, Permutation al (f al) /\ sorted (f al).
+  forall (al : list nat), Permutation al (f al) /\ sorted (f al).
